driver/IdSim.v
@@ -6,72 +6,232 @@ Require SoundTop UnreachC.
 Require SimSymbId SimSymbDrop.
 Require Import CoqlibC.
 Require Import ValuesC.
+Require Import Linking.
+Require Import MapsC.
+Require Import AxiomsC.
+Require Import Ord.
+Require Import MemoryC.
+Require Import SmallstepC.
 
 Set Implicit Arguments.
 
+
+Lemma match_program_refl
+      F V
+      `{Linker F} `{Linker V}
+      (prog: AST.program F V)
+  :
+    match_program (fun _ => eq) eq prog prog
+.
+Proof.
+  econs; eauto.
+  destruct prog; ss.
+  ginduction prog_defs; ii; ss.
+  { econs; eauto. }
+  destruct a; ss.
+  econs; eauto.
+  - econs; eauto. ss. destruct g; ss.
+    + econs; eauto. eapply linkorder_refl.
+    + econs; eauto. destruct v; ss.
+  - rpapply IHprog_defs; eauto.
+    apply Axioms.functional_extensionality. i.
+    destruct x; ss.
+    apply Axioms.functional_extensionality. i.
+    destruct x; ss.
+    apply prop_ext. split; ii.
+    + inv H1. ss. clarify. inv H3; econs; ss; eauto; econs; ss; eauto.
+      apply linkorder_refl.
+    + inv H1. ss. clarify. inv H3; econs; ss; eauto; econs; ss; eauto.
+      apply linkorder_refl.
+Unshelve.
+  all: ss.
+Qed.
+
 Local Existing Instance Val.mi_normal.
+Local Opaque Z.mul Z.add Z.sub Z.div.
 
 Parameter C_module: Csyntax.program -> Mod.t.
 
-Lemma tgt_id
-      (tgt: Asm.program)
+Lemma genv_eq
+      F V
+      (ge1 ge2: Genv.t F V)
+      (PUB: ge1.(Genv.genv_public) = ge2.(Genv.genv_public))
+      (NEXT: ge1.(Genv.genv_next) = ge2.(Genv.genv_next))
+      (SYMB: ge1.(Genv.genv_symb) = ge2.(Genv.genv_symb))
+      (DEFS: ge1.(Genv.genv_defs) = ge2.(Genv.genv_defs))
+  :
+    ge1 = ge2
+.
+Proof.
+  destruct ge1, ge2; ss. clarify.
+  f_equal.
+  - apply proof_irr.
+  - apply proof_irr.
+  - apply proof_irr.
+Qed.
+
+Lemma sim_skenv_eq
+      skenv_link_src skenv_link_tgt
+      (SKE: SimSymbId.sim_skenv skenv_link_src skenv_link_tgt)
+  :
+    skenv_link_src = skenv_link_tgt
+.
+Proof.
+  inv SKE; ss.
+  apply genv_eq; ss.
+  -
+Abort.
+
+
+
+Local Existing Instance SimMemId.SimMemId | 0.
+Local Existing Instance SimMemId.SimSymbId | 0.
+Local Existing Instance SoundTop.Top | 0.
+
+Lemma asm_id
+      (asm: Asm.program)
   :
     exists mp,
       (<<SIM: @ModPair.sim SimMemId.SimMemId SimMemId.SimSymbId SoundTop.Top mp>>)
-      /\ (<<SRC: mp.(ModPair.src) = tgt.(AsmC.module)>>)
-      /\ (<<TGT: mp.(ModPair.tgt) = tgt.(AsmC.module)>>)
+      /\ (<<SRC: mp.(ModPair.src) = asm.(AsmC.module)>>)
+      /\ (<<TGT: mp.(ModPair.tgt) = asm.(AsmC.module)>>)
 .
 Proof.
-  admit "this should hold".
+  eexists (ModPair.mk _ _ _); s.
+  assert(PROGSKEL: match_program (fun _ => eq) eq (Sk.of_program fn_sig asm) (Sk.of_program fn_sig asm)).
+  { econs; eauto. ss. eapply match_program_refl; eauto. }
+  assert(PROG: match_program (fun _ => eq) eq asm asm).
+  { econs; eauto. ss. eapply match_program_refl; eauto. }
+  esplits; eauto.
+  econs; ss; eauto.
+  ii. inv SSLE. clear_tac.
+
+  econs; ss; eauto.
+  { eapply SoundTop.sound_state_local_preservation; eauto. }
+  ii; ss.
+
+  exploit (SimSymbId.sim_skenv_revive PROG); try apply SIMSKENV; eauto.
+  (* hexploit (SimSymbId.sim_skenv_revive PROG). *)
+  { i; ss. clarify. }
+  (* { instantiate (1:= (SkEnv.project skenv_link_src (defs asm))). eauto. } *)
+  (* { instantiate (1:= (SkEnv.project skenv_link_tgt (defs asm))). eauto. } *)
+  (* { ss. } *)
+  intro GENV; des.
+
+  inv SIMARGS. destruct args_src, args_tgt; ss. clarify. destruct sm_arg; ss. clarify.
+  fold fundef in *.
+  split; ii; cycle 1.
+  { des. exists st_init_src. inv SAFESRC. econs; ss; eauto.
+    - unfold Genv.find_funct, Genv.find_funct_ptr in *. des_ifs_safe. inv GENV.
+      specialize (mge_defs b).
+      Local Opaque SkEnv.revive SkEnv.project.
+      unfold Genv.find_def in *. ss. rewrite Heq2 in *.
+      inv mge_defs; ss; clarify.
+      inv H1. ss.
+    - etrans; eauto.
+      admit "ez".
+  }
+  rename tgt into m0.
+  rename st_init_tgt into st0.
+  esplits; eauto.
+  { instantiate (1:= st0). clear SAFESRC.
+    inv INITTGT. econs; ss; eauto.
+    + unfold Genv.find_funct, Genv.find_funct_ptr in *. des_ifs_safe. inv GENV.
+      specialize (mge_defs b).
+      Local Opaque SkEnv.revive SkEnv.project.
+      unfold Genv.find_def in *. ss. rewrite Heq2 in *.
+      inv mge_defs; ss; clarify.
+      inv H1. ss.
+    + etrans; eauto. admit "ez".
+  }
+  instantiate (1:= (SimMemId.mk m0 m0)). instantiate (1:= Ord.lift_idx unit_ord_wf tt).
+  clear - GENV.
+  generalize dependent st0.
+  pcofix CIH. ii. pfold.
+  destruct (classic ((modsem skenv_link_src asm).(ModSem.is_call) st0)).
+  { ss. rr in H. des.
+    econs 3; eauto.
+    { econs; eauto. }
+    ii. des. clear_tac.
+    exists args_src. exists (SimMemId.mk args_src.(Args.m) args_src.(Args.m)). ss.
+    esplits; eauto.
+    { econs; ss; eauto. }
+    { admit "ez". }
+    ii. ss. des.
+    esplits; eauto.
+    admit "ez".
+  }
+  destruct (classic ((modsem skenv_link_src asm).(ModSem.is_return) st0)).
+  { ss. rr in H0. des.
+    dup H0. set (R:= retv). inv H0.
+    econs 4; eauto.
+    { instantiate (1:= SimMemId.mk m2 m2). ss. }
+    { econs; eauto. }
+    { ss. instantiate (1:= R). admit "ez". }
+    { ss. }
+  }
+  econs 1; eauto.
+  ii; des. clear_tac.
+  esplits; eauto.
+  econs; eauto; cycle 1.
+  { admit "ez". }
+  ii. ss. inv STEPSRC.
+  esplits; eauto. left. apply plus_one. econs; eauto.
+  { admit "ez". }
+  econs; eauto. ss. admit "ez".
+Unshelve.
+  all: ss.
 Qed.
 
-Lemma tgt_ext_top
-      (tgt: Asm.program)
+Lemma asm_ext_top
+      (asm: Asm.program)
   :
     exists mp,
       (<<SIM: @ModPair.sim SimMemExt.SimMemExt SimMemExt.SimSymbExtends SoundTop.Top mp>>)
-      /\ (<<SRC: mp.(ModPair.src) = tgt.(AsmC.module)>>)
-      /\ (<<TGT: mp.(ModPair.tgt) = tgt.(AsmC.module)>>)
+      /\ (<<SRC: mp.(ModPair.src) = asm.(AsmC.module)>>)
+      /\ (<<TGT: mp.(ModPair.tgt) = asm.(AsmC.module)>>)
 .
 Proof.
   admit "this should hold".
 Qed.
 
-Lemma tgt_ext_unreach
-      (tgt: Asm.program)
+Lemma asm_ext_unreach
+      (asm: Asm.program)
   :
     exists mp,
       (<<SIM: @ModPair.sim SimMemExt.SimMemExt SimMemExt.SimSymbExtends UnreachC.Unreach mp>>)
-      /\ (<<SRC: mp.(ModPair.src) = tgt.(AsmC.module)>>)
-      /\ (<<TGT: mp.(ModPair.tgt) = tgt.(AsmC.module)>>)
+      /\ (<<SRC: mp.(ModPair.src) = asm.(AsmC.module)>>)
+      /\ (<<TGT: mp.(ModPair.tgt) = asm.(AsmC.module)>>)
 .
 Proof.
   admit "this should hold".
 Qed.
 
-Lemma tgt_inj_id
+Lemma asm_inj_id
       (tgt: Asm.program)
   :
     exists mp,
       (<<SIM: @ModPair.sim SimMemInj.SimMemInj SimMemInj.SimSymbId SoundTop.Top mp>>)
-      /\ (<<SRC: mp.(ModPair.src) = tgt.(AsmC.module)>>)
-      /\ (<<TGT: mp.(ModPair.tgt) = tgt.(AsmC.module)>>)
+      /\ (<<SRC: mp.(ModPair.src) = asm.(AsmC.module)>>)
+      /\ (<<TGT: mp.(ModPair.tgt) = asm.(AsmC.module)>>)
 .
 Proof.
   admit "this should hold".
 Qed.
 
-Lemma tgt_inj_drop
+Lemma asm_inj_drop
       (tgt: Asm.program)
   :
     exists mp,
       (<<SIM: @ModPair.sim SimMemInj.SimMemInj SimSymbDrop.SimSymbDrop SoundTop.Top mp>>)
-      /\ (<<SRC: mp.(ModPair.src) = tgt.(AsmC.module)>>)
-      /\ (<<TGT: mp.(ModPair.tgt) = tgt.(AsmC.module)>>)
+      /\ (<<SRC: mp.(ModPair.src) = asm.(AsmC.module)>>)
+      /\ (<<TGT: mp.(ModPair.tgt) = asm.(AsmC.module)>>)
 .
 Proof.
   admit "this should hold".
 Qed.
+
+
 
 
 
