lib/CoqlibC.v
@@ -1027,3 +1027,11 @@ Qed.
 
 Global Opaque Z.mul.
 
+Lemma unit_ord_wf
+  :
+    well_founded (bot2: unit -> unit -> Prop)
+.
+Proof.
+  ii. induction a; ii; ss.
+Qed.
+
